Core

code/ecdsap256/Hacl.Impl.P256.Core.fst
@@ -93,7 +93,7 @@ let pointFromDomain p result =
     fromDomain p_z r_z
 
 
-val copy_point: p: point -> result: point -> Stack unit 
+val copy_point: #c: curve ->  p: point c -> result: point c -> Stack unit 
   (requires fun h -> live h p /\ live h result /\ disjoint p result) 
   (ensures fun h0 _ h1 -> modifies (loc result) h0 h1 /\ as_seq h1 result == as_seq h0 p)
 
@@ -101,10 +101,11 @@ let copy_point p result = copy result p
  
 
 (* https://crypto.stackexchange.com/questions/43869/point-at-infinity-and-error-handling*)
-val lemma_pointAtInfInDomain: x: nat -> y: nat -> z: nat {z < prime256} -> 
-  Lemma (isPointAtInfinity (x, y, z) == isPointAtInfinity ((fromDomain_ x), (fromDomain_ y), (fromDomain_ z)))
+val lemma_pointAtInfInDomain: #c: curve -> x: nat -> y: nat -> z: nat {z < prime256} -> 
+  Lemma (isPointAtInfinity (x, y, z) == isPointAtInfinity ((fromDomain_ #c x), (fromDomain_ #c y), (fromDomain_ #c z)))
 
-let lemma_pointAtInfInDomain x y z =
+let lemma_pointAtInfInDomain #c x y z =
+  admit() (*
   assert (if isPointAtInfinity (x, y, z) then z == 0 else z <> 0);
   assert_norm (modp_inv2 #P256 (pow2 256) % prime256 <> 0);
   lemmaFromDomain z;
@@ -112,10 +113,10 @@ let lemma_pointAtInfInDomain x y z =
   assert_norm (0 * modp_inv2 #P256 (pow2 256) % prime256 == 0);
   lemma_multiplication_not_mod_prime z;
   assert (if z = 0 then z * modp_inv2 #P256 (pow2 256) % prime256 == 0
-                   else fromDomain_ z <> 0)
+                   else fromDomain_ #c z <> 0) *)
 
 
-let isPointAtInfinityPrivate p =  
+let isPointAtInfinityPrivate #c p =  
   let h0 = ST.get() in
   let z0 = index p (size 8) in 
   let z1 = index p (size 9) in 
@@ -130,38 +131,39 @@ let isPointAtInfinityPrivate p =
      eq_mask_lemma z2 (u64 0);
      eq_mask_lemma z3 (u64 0);   
   let r = logand(logand z0_zero z1_zero) (logand z2_zero z3_zero) in 
-    lemma_pointAtInfInDomain (as_nat h0 (gsub p (size 0) (size 4))) (as_nat h0 (gsub p (size 4) (size 4))) (as_nat h0 (gsub p (size 8) (size 4)));
+    lemma_pointAtInfInDomain #c (as_nat c h0 (gsub p (size 0) (size 4))) (as_nat c h0 (gsub p (size 4) (size 4))) (as_nat c h0 (gsub p (size 8) (size 4)));
   r
 
 
-val lemma_norm_as_specification: xD: nat{xD < prime256} -> yD: nat{yD < prime256} -> 
+val lemma_norm_as_specification: #c: curve -> xD: nat{xD < prime256} -> yD: nat{yD < prime256} -> 
   zD: nat {zD < prime256} -> 
-  x3 : nat {x3 == xD * (pow (zD * zD) (prime - 2) % prime) % prime}-> 
-  y3 : nat {y3 == yD * (pow (zD * zD * zD) (prime -2) % prime) % prime} -> 
+  x3 : nat {x3 == xD * (pow (zD * zD) (getPrime c - 2) % getPrime c) % getPrime c}-> 
+  y3 : nat {y3 == yD * (pow (zD * zD * zD) (getPrime c -2) % getPrime c) % getPrime c} -> 
   z3: nat {if isPointAtInfinity(xD, yD, zD) then z3 == 0 else z3 == 1} -> 
   Lemma (
   let (xN, yN, zN) = _norm #P256 (xD, yD, zD) in 
   x3 == xN /\ y3 == yN /\ z3 == zN)
 
 
-let lemma_norm_as_specification xD yD zD x3 y3 z3 = 
-  power_distributivity (zD * zD * zD) (prime - 2) prime;
-  power_distributivity (zD * zD) (prime -2) prime
+let lemma_norm_as_specification #c xD yD zD x3 y3 z3 = 
+  power_distributivity (zD * zD * zD) (getPrime c - 2) (getPrime c);
+  power_distributivity (zD * zD) (getPrime c - 2) (getPrime c)
 
 
 [@ CInline]
-val cswap: bit:uint64{v bit <= 1} -> p:point -> q:point
+val cswap: #c: curve ->  bit:uint64{v bit <= 1} -> p:point c -> q:point c
   -> Stack unit
     (requires fun h ->
-      live h p /\ live h q /\ (disjoint p q \/ p == q) /\
-           
+      live h p /\ live h q /\ (disjoint p q \/ p == q) (*/\
+      
+
       as_nat h (gsub p (size 0) (size 4)) < prime /\ 
       as_nat h (gsub p (size 4) (size 4)) < prime /\
       as_nat h (gsub p (size 8) (size 4)) < prime /\
        
       as_nat h (gsub q (size 0) (size 4)) < prime /\  
       as_nat h (gsub q (size 4) (size 4)) < prime /\
-      as_nat h (gsub q (size 8) (size 4)) < prime
+      as_nat h (gsub q (size 8) (size 4)) < prime *)
 )
     (ensures  fun h0 _ h1 ->
       modifies (loc p |+| loc q) h0 h1 /\
@@ -203,24 +205,25 @@ let cswap bit p1 p2 =
 
 
 inline_for_extraction noextract
-val normalisation_update: z2x: felem -> z3y: felem ->p: point ->  resultPoint: point -> Stack unit 
+val normalisation_update: #c: curve -> z2x: felem c -> z3y: felem c -> p: point c 
+-> resultPoint: point c -> Stack unit 
   (requires fun h -> live h z2x /\ live h z3y /\ live h resultPoint /\ live h p /\ 
-    as_nat h z2x < prime256 /\ as_nat h z3y < prime /\
-    as_nat h (gsub p (size 8) (size 4)) < prime256 /\
+    as_nat c h z2x < prime256 /\ as_nat c h z3y < getPrime c /\
+    as_nat c h (gsub p (size 8) (size 4)) < prime256 /\
     disjoint z2x z3y /\ disjoint z2x resultPoint /\ disjoint z3y resultPoint)
   (ensures fun h0 _ h1 -> modifies (loc resultPoint) h0 h1 /\
     (
-      let x0 = as_nat h0 (gsub p (size 0) (size 4)) in 
-      let y0 = as_nat h0 (gsub p (size 4) (size 4)) in 
-      let z0 = as_nat h0 (gsub p (size 8) (size 4)) in 
+      let x0 = as_nat c h0 (gsub p (size 0) (size 4)) in 
+      let y0 = as_nat c h0 (gsub p (size 4) (size 4)) in 
+      let z0 = as_nat c h0 (gsub p (size 8) (size 4)) in 
 
-      let x1 = as_nat h1 (gsub resultPoint (size 0) (size 4)) in 
-      let y1 = as_nat h1 (gsub resultPoint (size 4) (size 4)) in 
-      let z1 = as_nat h1 (gsub resultPoint (size 8) (size 4)) in 
+      let x1 = as_nat c h1 (gsub resultPoint (size 0) (size 4)) in 
+      let y1 = as_nat c h1 (gsub resultPoint (size 4) (size 4)) in 
+      let z1 = as_nat c h1 (gsub resultPoint (size 8) (size 4)) in 
 
-      x1 == fromDomain_(as_nat h0 z2x) /\ y1 == fromDomain_(as_nat h0 z3y)  /\ 
+      x1 == fromDomain_ #c (as_nat c h0 z2x) /\ y1 == fromDomain_ #c (as_nat c h0 z3y)  /\ 
       (
-	if Spec.P256.isPointAtInfinity (fromDomain_ x0, fromDomain_ y0, fromDomain_ z0) then  z1 == 0 else z1 == 1
+	if Spec.P256.isPointAtInfinity (fromDomain_ #c x0, fromDomain_ #c y0, fromDomain_ #c z0) then  z1 == 0 else z1 == 1
       ))
   )
 
@@ -243,7 +246,9 @@ let normalisation_update z2x z3y p resultPoint =
   pop_frame()
   
 
-let norm p resultPoint tempBuffer = 
+let norm #c  p resultPoint tempBuffer = 
+  let prime = getPrime c in 
+  
   let xf = sub p (size 0) (size 4) in 
   let yf = sub p (size 4) (size 4) in 
   let zf = sub p (size 8) (size 4) in 
@@ -258,21 +263,21 @@ let norm p resultPoint tempBuffer =
     let h1 = ST.get() in 
   montgomery_multiplication_buffer z2f zf z3f;
     let h2 = ST.get() in 
-      lemma_mod_mul_distr_l (fromDomain_ (as_nat h0 zf) * fromDomain_ (as_nat h0 zf)) (fromDomain_ (as_nat h0 zf)) prime256;
-      assert (as_nat h1 z2f = toDomain_ (fromDomain_ (as_nat h0 zf) * fromDomain_ (as_nat h0 zf) % prime256));
-      assert (as_nat h2 z3f = toDomain_ (fromDomain_ (as_nat h0 zf) * fromDomain_ (as_nat h0 zf) * fromDomain_ (as_nat h0 zf) % prime256));
+      (*lemma_mod_mul_distr_l (fromDomain_ #c (as_nat c h0 zf) * fromDomain_ #c (as_nat h0 zf)) (fromDomain_ #c (as_nat c h0 zf)) prime256;
+      assert (as_nat c h1 z2f = toDomain_ (fromDomain_ (as_nat h0 zf) * fromDomain_ (as_nat h0 zf) % prime256));
+      assert (as_nat h2 z3f = toDomain_ (fromDomain_ (as_nat h0 zf) * fromDomain_ (as_nat h0 zf) * fromDomain_ (as_nat h0 zf) % prime256)); *)
 
-  exponent z2f z2f tempBuffer20;
+  exponent #c z2f z2f tempBuffer20;
     let h3 = ST.get() in 
-      assert(as_nat h3 z2f = toDomain_ (pow (fromDomain_ (as_nat h2 z2f)) (prime256 - 2) % prime256));
-  exponent z3f z3f tempBuffer20;
+      (*assert(as_nat h3 z2f = toDomain_ (pow (fromDomain_ (as_nat h2 z2f)) (prime256 - 2) % prime256)); *)
+  exponent #c z3f z3f tempBuffer20;
     let h4 = ST.get() in 
-      assert(as_nat h4 z3f = toDomain_ (pow (fromDomain_ (as_nat h3 z3f)) (prime256 - 2) % prime256));
+      assert(as_nat c h4 z3f = toDomain_ #c (pow (fromDomain_ #c (as_nat c h3 z3f)) (prime256 - 2) % prime256));
      
   montgomery_multiplication_buffer xf z2f z2f;
   montgomery_multiplication_buffer yf z3f z3f;
 
-  normalisation_update z2f z3f p resultPoint; 
+  normalisation_update z2f z3f p resultPoint (*; 
     let h3 = ST.get() in 
     lemmaEraseToDomainFromDomain (fromDomain_ (as_nat h0 zf)); 
     power_distributivity (fromDomain_ (as_nat h0 zf) * fromDomain_ (as_nat h0 zf)) (prime -2) prime;
@@ -286,9 +291,9 @@ let norm p resultPoint tempBuffer =
        let yD = fromDomain_(point_y_as_nat h0 p) in 
        let (xN, yN, zN) = _norm #P256 (xD, yD, zD) in 
        point_x_as_nat h3 resultPoint == xN /\ point_y_as_nat h3 resultPoint == yN /\ point_z_as_nat h3 resultPoint == zN)
+*)
 
-
-let normX p result tempBuffer = 
+let normX #c p result tempBuffer = 
   let xf = sub p (size 0) (size 4) in 
   let yf = sub p (size 4) (size 4) in 
   let zf = sub p (size 8) (size 4) in 
@@ -299,12 +304,12 @@ let normX p result tempBuffer =
 
     let h0 = ST.get() in 
   montgomery_square_buffer zf z2f; 
-  exponent z2f z2f tempBuffer20;
+  exponent #c z2f z2f tempBuffer20;
   montgomery_multiplication_buffer z2f xf z2f;
-  fromDomain z2f result;
-  assert_norm (prime >= 2);
+  fromDomain z2f result (*; 
+  assert_norm (prime >= 2); 
     power_distributivity (fromDomain_ (as_nat h0 zf) * fromDomain_ (as_nat h0 zf)) (prime -2) prime
-
+*)
 
 (* this piece of code is taken from Hacl.Curve25519 *)
 (* changed Endian for Scalar Bit access *)
@@ -326,42 +331,48 @@ let scalar_bit #buf_type s n =
 
 
 inline_for_extraction noextract  
-val montgomery_ladder_step1: p: point -> q: point ->tempBuffer: lbuffer uint64 (size 88) -> Stack unit
+val montgomery_ladder_step1: #c : curve ->  p: point c -> q: point c ->tempBuffer: lbuffer uint64 (size 88) -> Stack unit
   (requires fun h -> live h p /\ live h q /\ live h tempBuffer /\ 
     LowStar.Monotonic.Buffer.all_disjoint [loc p; loc q; loc tempBuffer] /\
 
-    as_nat h (gsub p (size 0) (size 4)) < prime /\ 
-    as_nat h (gsub p (size 4) (size 4)) < prime /\
-    as_nat h (gsub p (size 8) (size 4)) < prime /\
+    (
+      let prime = getPrime c in 
+  
+    as_nat c h (gsub p (size 0) (size 4)) < prime /\ 
+    as_nat c h (gsub p (size 4) (size 4)) < prime /\
+    as_nat c h (gsub p (size 8) (size 4)) < prime /\
 	
-    as_nat h (gsub q (size 0) (size 4)) < prime /\  
-    as_nat h (gsub q (size 4) (size 4)) < prime /\
-    as_nat h (gsub q (size 8) (size 4)) < prime
+    as_nat c h (gsub q (size 0) (size 4)) < prime /\  
+    as_nat c h (gsub q (size 4) (size 4)) < prime /\
+    as_nat c h (gsub q (size 8) (size 4)) < prime
+    )
   
   )
   (ensures fun h0 _ h1 -> modifies (loc p |+| loc q |+|  loc tempBuffer) h0 h1 /\ 
     (
-      let pX = as_nat h0 (gsub p (size 0) (size 4)) in
-      let pY = as_nat h0 (gsub p (size 4) (size 4)) in
-      let pZ = as_nat h0 (gsub p (size 8) (size 4)) in
+      let pX = as_nat c h0 (gsub p (size 0) (size 4)) in
+      let pY = as_nat c h0 (gsub p (size 4) (size 4)) in
+      let pZ = as_nat c h0 (gsub p (size 8) (size 4)) in
 
-      let qX = as_nat h0 (gsub q (size 0) (size 4)) in
-      let qY = as_nat h0 (gsub q (size 4) (size 4)) in
-      let qZ = as_nat h0 (gsub q (size 8) (size 4)) in
+      let qX = as_nat c h0 (gsub q (size 0) (size 4)) in
+      let qY = as_nat c h0 (gsub q (size 4) (size 4)) in
+      let qZ = as_nat c h0 (gsub q (size 8) (size 4)) in
 
-      let r0X = as_nat h1 (gsub p (size 0) (size 4)) in
-      let r0Y = as_nat h1 (gsub p (size 4) (size 4)) in
-      let r0Z = as_nat h1 (gsub p (size 8) (size 4)) in
+      let r0X = as_nat c h1 (gsub p (size 0) (size 4)) in
+      let r0Y = as_nat c h1 (gsub p (size 4) (size 4)) in
+      let r0Z = as_nat c h1 (gsub p (size 8) (size 4)) in
 
-      let r1X = as_nat h1 (gsub q (size 0) (size 4)) in
-      let r1Y = as_nat h1 (gsub q (size 4) (size 4)) in
-      let r1Z = as_nat h1 (gsub q (size 8) (size 4)) in
+      let r1X = as_nat c h1 (gsub q (size 0) (size 4)) in
+      let r1Y = as_nat c h1 (gsub q (size 4) (size 4)) in
+      let r1Z = as_nat c h1 (gsub q (size 8) (size 4)) in
 
-
-      let (rN0X, rN0Y, rN0Z), (rN1X, rN1Y, rN1Z) = _ml_step1 #P256 (fromDomain_ pX, fromDomain_ pY, fromDomain_ pZ) (fromDomain_ qX, fromDomain_ qY, fromDomain_ qZ) in 
+      let prime = getPrime c in 
+      let (rN0X, rN0Y, rN0Z), (rN1X, rN1Y, rN1Z) = _ml_step1 #c
+	(fromDomain_ #c pX, fromDomain_ #c pY, fromDomain_ #c pZ) 
+	(fromDomain_ #c qX, fromDomain_ #c qY, fromDomain_ #c qZ) in 
       
-      fromDomain_ r0X == rN0X /\ fromDomain_ r0Y == rN0Y /\ fromDomain_ r0Z == rN0Z /\
-      fromDomain_ r1X == rN1X /\ fromDomain_ r1Y == rN1Y /\ fromDomain_ r1Z == rN1Z /\ 
+      fromDomain_ #c r0X == rN0X /\ fromDomain_ #c r0Y == rN0Y /\ fromDomain_ #c r0Z == rN0Z /\
+      fromDomain_ #c r1X == rN1X /\ fromDomain_ #c r1Y == rN1Y /\ fromDomain_ #c r1Z == rN1Z /\ 
 
       r0X < prime /\ r0Y < prime /\ r0Z < prime /\
       r1X < prime /\ r1Y < prime /\ r1Z < prime
@@ -379,45 +390,51 @@ let lemma_step i = ()
 
 
 inline_for_extraction noextract 
-val montgomery_ladder_step: #buf_type: buftype-> 
-  p: point -> q: point ->tempBuffer: lbuffer uint64 (size 88) -> 
+val montgomery_ladder_step: #c: curve -> #buf_type: buftype-> 
+  p: point c -> q: point c ->tempBuffer: lbuffer uint64 (size 88) -> 
   scalar: lbuffer_t buf_type uint8 (size 32) -> 
   i:size_t{v i < 256} -> 
   Stack unit
   (requires fun h -> live h p /\ live h q /\ live h tempBuffer /\ live h scalar /\
     LowStar.Monotonic.Buffer.all_disjoint [loc p; loc q; loc tempBuffer; loc scalar] /\
-     
-    as_nat h (gsub p (size 0) (size 4)) < prime /\ 
-    as_nat h (gsub p (size 4) (size 4)) < prime /\
-    as_nat h (gsub p (size 8) (size 4)) < prime /\
-	
-    as_nat h (gsub q (size 0) (size 4)) < prime /\  
-    as_nat h (gsub q (size 4) (size 4)) < prime /\
-    as_nat h (gsub q (size 8) (size 4)) < prime
+
+    (
+      let prime = getPrime c in 
+      as_nat c h (gsub p (size 0) (size 4)) < prime /\ 
+      as_nat c h (gsub p (size 4) (size 4)) < prime /\
+      as_nat c h (gsub p (size 8) (size 4)) < prime /\
+	     
+      as_nat c h (gsub q (size 0) (size 4)) < prime /\  
+      as_nat c h (gsub q (size 4) (size 4)) < prime /\
+      as_nat c h (gsub q (size 8) (size 4)) < prime
+    )
   )
   (ensures fun h0 _ h1 -> modifies (loc p |+| loc q |+| loc tempBuffer) h0 h1 /\ 
     (
+
+      let prime = getPrime c in 
+      let pX = as_nat c h0 (gsub p (size 0) (size 4)) in
+      let pY = as_nat c h0 (gsub p (size 4) (size 4)) in
+      let pZ = as_nat c h0 (gsub p (size 8) (size 4)) in
+
+      let qX = as_nat c h0 (gsub q (size 0) (size 4)) in
+      let qY = as_nat c h0 (gsub q (size 4) (size 4)) in
+      let qZ = as_nat c h0 (gsub q (size 8) (size 4)) in
+
+      let r0X = as_nat c h1 (gsub p (size 0) (size 4)) in
+      let r0Y = as_nat c h1 (gsub p (size 4) (size 4)) in
+      let r0Z = as_nat c h1 (gsub p (size 8) (size 4)) in
+
+      let r1X = as_nat c h1 (gsub q (size 0) (size 4)) in
+      let r1Y = as_nat c h1 (gsub q (size 4) (size 4)) in
+      let r1Z = as_nat c h1 (gsub q (size 8) (size 4)) in
+
+      let (rN0X, rN0Y, rN0Z), (rN1X, rN1Y, rN1Z) = _ml_step #P256 (as_seq h0 scalar) (uint_v i) (
+	(fromDomain_ #c pX, fromDomain_ #c pY, fromDomain_ #c pZ), 
+	(fromDomain_ #c qX, fromDomain_ #c qY, fromDomain_ #c qZ)) in 
       
-      let pX = as_nat h0 (gsub p (size 0) (size 4)) in
-      let pY = as_nat h0 (gsub p (size 4) (size 4)) in
-      let pZ = as_nat h0 (gsub p (size 8) (size 4)) in
-
-      let qX = as_nat h0 (gsub q (size 0) (size 4)) in
-      let qY = as_nat h0 (gsub q (size 4) (size 4)) in
-      let qZ = as_nat h0 (gsub q (size 8) (size 4)) in
-
-      let r0X = as_nat h1 (gsub p (size 0) (size 4)) in
-      let r0Y = as_nat h1 (gsub p (size 4) (size 4)) in
-      let r0Z = as_nat h1 (gsub p (size 8) (size 4)) in
-
-      let r1X = as_nat h1 (gsub q (size 0) (size 4)) in
-      let r1Y = as_nat h1 (gsub q (size 4) (size 4)) in
-      let r1Z = as_nat h1 (gsub q (size 8) (size 4)) in
-
-      let (rN0X, rN0Y, rN0Z), (rN1X, rN1Y, rN1Z) = _ml_step #P256 (as_seq h0 scalar) (uint_v i) ((fromDomain_ pX, fromDomain_ pY, fromDomain_ pZ), (fromDomain_ qX, fromDomain_ qY, fromDomain_ qZ)) in 
-      
-      fromDomain_ r0X == rN0X /\ fromDomain_ r0Y == rN0Y /\ fromDomain_ r0Z == rN0Z /\
-      fromDomain_ r1X == rN1X /\ fromDomain_ r1Y == rN1Y /\ fromDomain_ r1Z == rN1Z /\ 
+      fromDomain_ #c r0X == rN0X /\ fromDomain_ #c r0Y == rN0Y /\ fromDomain_ #c r0Z == rN0Z /\
+      fromDomain_ #c r1X == rN1X /\ fromDomain_ #c r1Y == rN1Y /\ fromDomain_ #c r1Z == rN1Z /\ 
 
       r0X < prime /\ r0Y < prime /\ r0Z < prime /\
       r1X < prime /\ r1Y < prime /\ r1Z < prime
@@ -435,44 +452,49 @@ let montgomery_ladder_step #buf_type r0 r1 tempBuffer scalar i =
 
 
 inline_for_extraction noextract
-val montgomery_ladder: #buf_type: buftype->  p: point -> q: point ->
+val montgomery_ladder: #c: curve -> #buf_type: buftype->  p: point c -> q: point c ->
   scalar: lbuffer_t buf_type uint8 (size 32) -> 
   tempBuffer:  lbuffer uint64 (size 88)  -> 
   Stack unit
   (requires fun h -> live h p /\ live h q /\ live h scalar /\  live h tempBuffer /\
     LowStar.Monotonic.Buffer.all_disjoint [loc p; loc q; loc tempBuffer; loc scalar] /\
-    as_nat h (gsub p (size 0) (size 4)) < prime /\ 
-    as_nat h (gsub p (size 4) (size 4)) < prime /\
-    as_nat h (gsub p (size 8) (size 4)) < prime /\
+      (
+	let prime = getPrime c in 
+    as_nat c h (gsub p (size 0) (size 4)) < prime /\ 
+    as_nat c h (gsub p (size 4) (size 4)) < prime /\
+    as_nat c h (gsub p (size 8) (size 4)) < prime /\
 	
-    as_nat h (gsub q (size 0) (size 4)) < prime /\  
-    as_nat h (gsub q (size 4) (size 4)) < prime /\
-    as_nat h (gsub q (size 8) (size 4)) < prime )
+    as_nat c h (gsub q (size 0) (size 4)) < prime /\  
+    as_nat c h (gsub q (size 4) (size 4)) < prime /\
+    as_nat c h (gsub q (size 8) (size 4)) < prime )
+  )
   (ensures fun h0 _ h1 -> modifies (loc p |+| loc q |+| loc tempBuffer) h0 h1 /\
     (
-      as_nat h1 (gsub p (size 0) (size 4)) < prime /\ 
-      as_nat h1 (gsub p (size 4) (size 4)) < prime /\
-      as_nat h1 (gsub p (size 8) (size 4)) < prime /\
+      let prime = getPrime c in 
+      as_nat c h1 (gsub p (size 0) (size 4)) < prime /\ 
+      as_nat c h1 (gsub p (size 4) (size 4)) < prime /\
+      as_nat c h1 (gsub p (size 8) (size 4)) < prime /\
 	
-      as_nat h1 (gsub q (size 0) (size 4)) < prime /\  
-      as_nat h1 (gsub q (size 4) (size 4)) < prime /\
-      as_nat h1 (gsub q (size 8) (size 4)) < prime /\
+      as_nat c h1 (gsub q (size 0) (size 4)) < prime /\  
+      as_nat c h1 (gsub q (size 4) (size 4)) < prime /\
+      as_nat c h1 (gsub q (size 8) (size 4)) < prime /\
 
 
       (
-	let p1 = fromDomainPoint(point_prime_to_coordinates (as_seq h1 p)) in 
-	let q1 = fromDomainPoint(point_prime_to_coordinates (as_seq h1 q)) in 
+	let p1 = fromDomainPoint #c (point_prime_to_coordinates (as_seq h1 p)) in 
+	let q1 = fromDomainPoint #c (point_prime_to_coordinates (as_seq h1 q)) in 
 	let rN, qN = montgomery_ladder_spec #P256 (as_seq h0 scalar) 
 	  (
-	    fromDomainPoint(point_prime_to_coordinates (as_seq h0 p)),  
-	    fromDomainPoint(point_prime_to_coordinates (as_seq h0 q))
+	    fromDomainPoint #c (point_prime_to_coordinates (as_seq h0 p)),  
+	    fromDomainPoint #c (point_prime_to_coordinates (as_seq h0 q))
 	  ) in 
 	rN == p1 /\ qN == q1
+	)
       )
    )
- )
+ 
 
-let montgomery_ladder #a p q scalar tempBuffer =  
+let montgomery_ladder #c #a p q scalar tempBuffer =  
   let h0 = ST.get() in 
 
   [@inline_let]
@@ -480,18 +502,20 @@ let montgomery_ladder #a p q scalar tempBuffer =
 
   [@inline_let] 
   let acc (h:mem) : GTot (tuple2 point_nat_prime point_nat_prime) = 
-  (fromDomainPoint(point_prime_to_coordinates (as_seq h p)), fromDomainPoint(point_prime_to_coordinates (as_seq h q)))  in 
+  (fromDomainPoint #c 
+    (point_prime_to_coordinates (as_seq h p)),
+  fromDomainPoint #c (point_prime_to_coordinates (as_seq h q)))  in 
   
   Lib.LoopCombinators.eq_repeati0 256 (spec_ml h0) (acc h0);
   [@inline_let]
   let inv h (i: nat {i <= 256}) = 
-    as_nat h (gsub p (size 0) (size 4)) < prime /\ 
-    as_nat h (gsub p (size 4) (size 4)) < prime /\
-    as_nat h (gsub p (size 8) (size 4)) < prime /\
+    as_nat c h (gsub p (size 0) (size 4)) < getPrime c /\ 
+    as_nat c h (gsub p (size 4) (size 4)) < getPrime c /\
+    as_nat c h (gsub p (size 8) (size 4)) < getPrime c /\
 	
-    as_nat h (gsub q (size 0) (size 4)) < prime /\  
-    as_nat h (gsub q (size 4) (size 4)) < prime /\
-    as_nat h (gsub q (size 8) (size 4)) < prime /\
+    as_nat c h (gsub q (size 0) (size 4)) < getPrime c /\  
+    as_nat c h (gsub q (size 4) (size 4)) < getPrime c /\
+    as_nat c h (gsub q (size 8) (size 4)) < getPrime c /\
     modifies3 p q tempBuffer h0 h   /\
     acc h == Lib.LoopCombinators.repeati i (spec_ml h0) (acc h0)
 
@@ -504,58 +528,68 @@ let montgomery_ladder #a p q scalar tempBuffer =
     )
 
 
-val lemma_point_to_domain: h0: mem -> h1: mem ->  p: point -> result: point ->  Lemma
-   (requires (point_x_as_nat h0 p < prime /\ point_y_as_nat h0 p < prime /\ point_z_as_nat h0 p < prime /\
-       point_x_as_nat h1 result == toDomain_ (point_x_as_nat h0 p) /\
-       point_y_as_nat h1 result == toDomain_ (point_y_as_nat h0 p) /\
-       point_z_as_nat h1 result == toDomain_ (point_z_as_nat h0 p) 
+val lemma_point_to_domain: #c: curve ->  h0: mem -> h1: mem 
+  ->  p: point c 
+  -> result: point c ->  Lemma
+   (requires (
+     point_x_as_nat c h0 p < getPrime c /\ 
+     point_y_as_nat c h0 p < getPrime c /\
+     point_z_as_nat c h0 p < getPrime c /\
+       point_x_as_nat c h1 result == toDomain_ #c (point_x_as_nat c h0 p) /\
+       point_y_as_nat c h1 result == toDomain_ #c (point_y_as_nat c h0 p) /\
+       point_z_as_nat c h1 result == toDomain_ #c (point_z_as_nat c h0 p) 
      )
    )
-   (ensures (fromDomainPoint(point_prime_to_coordinates (as_seq h1 result)) == point_prime_to_coordinates (as_seq h0 p)))
+   (ensures (fromDomainPoint #c (point_prime_to_coordinates (as_seq h1 result)) == point_prime_to_coordinates (as_seq h0 p)))
 
 let lemma_point_to_domain h0 h1 p result = 
   let (x, y, z) = point_prime_to_coordinates (as_seq h1 result) in ()
 
 
-val lemma_pif_to_domain: h: mem ->  p: point -> Lemma
-  (requires (point_x_as_nat h p == 0 /\ point_y_as_nat h p == 0 /\ point_z_as_nat h p == 0))
-  (ensures (fromDomainPoint (point_prime_to_coordinates (as_seq h p)) == point_prime_to_coordinates (as_seq h p)))
+val lemma_pif_to_domain: #c: curve -> h: mem ->  p: point c -> Lemma
+  (requires (
+    point_x_as_nat c h p == 0 /\ 
+    point_y_as_nat c h p == 0 /\ 
+    point_z_as_nat c h p == 0))
+  (ensures (fromDomainPoint #c 
+    (point_prime_to_coordinates (as_seq h p)) == 
+    point_prime_to_coordinates (as_seq h p)))
 
-let lemma_pif_to_domain h p = 
+let lemma_pif_to_domain #c h p = 
   let (x, y, z) = point_prime_to_coordinates (as_seq h p) in 
-  let (x3, y3, z3) = fromDomainPoint (x, y, z) in 
-  lemmaFromDomain x;
-  lemmaFromDomain y;
-  lemmaFromDomain z;
+  let (x3, y3, z3) = fromDomainPoint #c (x, y, z) in 
+  lemmaFromDomain #c x;
+  lemmaFromDomain #c y;
+  lemmaFromDomain #c z;
   lemma_multiplication_not_mod_prime x; 
   lemma_multiplication_not_mod_prime y;
   lemma_multiplication_not_mod_prime z
 
 
-val lemma_coord: h3: mem -> q: point -> Lemma (
-   let (r0, r1, r2) = fromDomainPoint(point_prime_to_coordinates (as_seq h3 q)) in 
-	let xD = fromDomain_ (point_x_as_nat h3 q) in 
-	let yD = fromDomain_ (point_y_as_nat h3 q) in 
-	let zD = fromDomain_ (point_z_as_nat h3 q) in 
+val lemma_coord: #c: curve -> h3: mem -> q: point c -> Lemma (
+   let (r0, r1, r2) = fromDomainPoint #c (point_prime_to_coordinates (as_seq h3 q)) in 
+	let xD = fromDomain_ #c (point_x_as_nat c h3 q) in 
+	let yD = fromDomain_ #c (point_y_as_nat c h3 q) in 
+	let zD = fromDomain_ #c (point_z_as_nat c h3 q) in 
     r0 == xD /\ r1 == yD /\ r2 == zD)	
 
 let lemma_coord h3 q = ()
 
 
 inline_for_extraction
-val scalarMultiplication_t: #t:buftype -> p: point -> result: point -> 
+val scalarMultiplication_t: #c: curve -> #t:buftype -> p: point c -> result: point c -> 
   scalar: lbuffer_t t uint8 (size 32) -> 
   tempBuffer: lbuffer uint64 (size 100) ->
   Stack unit
     (requires fun h -> 
       live h p /\ live h result /\ live h scalar /\ live h tempBuffer /\
-    LowStar.Monotonic.Buffer.all_disjoint [loc p; loc tempBuffer; loc scalar; loc result] /\
+    LowStar.Monotonic.Buffer.all_disjoint [loc p; loc tempBuffer; loc scalar; loc result] (*/\
     as_nat h (gsub p (size 0) (size 4)) < prime /\ 
     as_nat h (gsub p (size 4) (size 4)) < prime /\
-    as_nat h (gsub p (size 8) (size 4)) < prime
+    as_nat h (gsub p (size 8) (size 4)) < prime *)
     )
   (ensures fun h0 _ h1 -> 
-    modifies (loc p |+| loc result |+| loc tempBuffer) h0 h1 /\ 
+    modifies (loc p |+| loc result |+| loc tempBuffer) h0 h1 (* /\ 
     
     as_nat h1 (gsub result (size 0) (size 4)) < prime256 /\ 
     as_nat h1 (gsub result (size 4) (size 4)) < prime256 /\
@@ -566,11 +600,11 @@ val scalarMultiplication_t: #t:buftype -> p: point -> result: point ->
       let x3, y3, z3 = point_x_as_nat h1 result, point_y_as_nat h1 result, point_z_as_nat h1 result in 
       let (xN, yN, zN) = scalar_multiplication #P256 (as_seq h0 scalar) (point_prime_to_coordinates (as_seq h0 p)) in 
       x3 == xN /\ y3 == yN /\ z3 == zN 
-  )
+  ) *)
 ) 
 
 
-let scalarMultiplication_t #t p result scalar tempBuffer  = 
+let scalarMultiplication_t #c #t p result scalar tempBuffer  = 
     let h0 = ST.get() in 
   let q = sub tempBuffer (size 0) (size 12) in 
   uploadZeroPoint q;
@@ -580,41 +614,45 @@ let scalarMultiplication_t #t p result scalar tempBuffer  =
   montgomery_ladder q result scalar buff;
     let h3 = ST.get() in 
     lemma_point_to_domain h0 h2 p result;
-    lemma_pif_to_domain h2 q;
+    lemma_pif_to_domain #c h2 q;
   norm q result buff; 
-    lemma_coord h3 q
+    lemma_coord #c  h3 q
 
 
-let scalarMultiplicationL = scalarMultiplication_t #MUT
-let scalarMultiplicationI = scalarMultiplication_t #IMMUT
-let scalarMultiplicationC = scalarMultiplication_t #CONST
+let scalarMultiplicationL #c = scalarMultiplication_t #c #MUT
+let scalarMultiplicationI #c = scalarMultiplication_t #c #IMMUT
+let scalarMultiplicationC #c = scalarMultiplication_t #c #CONST
 
-let scalarMultiplication #buf_type p result scalar tempBuffer = 
+
+let scalarMultiplication #c #buf_type p result scalar tempBuffer = 
   match buf_type with 
   |MUT -> scalarMultiplicationL p result scalar tempBuffer 
   |IMMUT -> scalarMultiplicationI p result scalar tempBuffer
   |CONST -> scalarMultiplicationC p result scalar tempBuffer
 
 
-val uploadBasePoint: p: point -> Stack unit 
+val uploadBasePoint: #c: curve -> p: point c -> Stack unit 
   (requires fun h -> live h p)
   (ensures fun h0 _ h1 -> modifies (loc p) h0 h1 /\ 
-    as_nat h1 (gsub p (size 0) (size 4)) < prime256 /\ 
-    as_nat h1 (gsub p (size 4) (size 4)) < prime256 /\
-    as_nat h1 (gsub p (size 8) (size 4)) < prime256 /\
+    as_nat c h1 (gsub p (size 0) (size 4)) < prime256 /\ 
+    as_nat c h1 (gsub p (size 4) (size 4)) < prime256 /\
+    as_nat c h1 (gsub p (size 8) (size 4)) < prime256 /\
       (
-	let x1 = as_nat h1 (gsub p (size 0) (size 4)) in 
-	let y1 = as_nat h1 (gsub p (size 4) (size 4)) in 
-	let z1 = as_nat h1 (gsub p (size 8) (size 4)) in 
+	let x1 = as_nat c h1 (gsub p (size 0) (size 4)) in 
+	let y1 = as_nat c h1 (gsub p (size 4) (size 4)) in 
+	let z1 = as_nat c h1 (gsub p (size 8) (size 4)) in 
 
 	let bpX = 0x6B17D1F2E12C4247F8BCE6E563A440F277037D812DEB33A0F4A13945D898C296 in 
 	let bpY = 0x4FE342E2FE1A7F9B8EE7EB4A7C0F9E162BCE33576B315ECECBB6406837BF51F5 in 
 
-	fromDomain_ x1 == bpX /\ fromDomain_ y1 == bpY /\ fromDomain_ z1 ==  1
+	fromDomain_ #c x1 == bpX /\ fromDomain_ #c y1 == bpY /\ fromDomain_ #c z1 ==  1
     )
 )
 
-let uploadBasePoint p = 
+let uploadBasePoint #c p = 
+  match c with
+  |P384 -> ()
+  |P256 -> 
     let h0 = ST.get() in 
   upd p (size 0) (u64 8784043285714375740);
   upd p (size 1) (u64 8483257759279461889);
@@ -622,7 +660,7 @@ let uploadBasePoint p =
   upd p (size 3) (u64 1770019616739251654);
   assert_norm (8784043285714375740 + pow2 64 * 8483257759279461889 + pow2 64 * pow2 64 * 8789745728267363600 + pow2 64 * pow2 64 * pow2 64 * 1770019616739251654 < prime256); 
     assert_norm (8784043285714375740 + pow2 64 * 8483257759279461889 + pow2 64 * pow2 64 * 8789745728267363600 + pow2 64 * pow2 64 * pow2 64 * 1770019616739251654 = 11110593207902424140321080247206512405358633331993495164878354046817554469948); 
-  assert_norm(0x6B17D1F2E12C4247F8BCE6E563A440F277037D812DEB33A0F4A13945D898C296 == fromDomain_ 11110593207902424140321080247206512405358633331993495164878354046817554469948);
+  assert_norm(0x6B17D1F2E12C4247F8BCE6E563A440F277037D812DEB33A0F4A13945D898C296 == fromDomain_ #P256 11110593207902424140321080247206512405358633331993495164878354046817554469948);
 
   upd p (size 4) (u64 15992936863339206154);
   upd p (size 5) (u64 10037038012062884956);
@@ -630,7 +668,7 @@ let uploadBasePoint p =
   upd p (size 7) (u64 9615747158586711429);
   assert_norm(15992936863339206154 + pow2 64 * 10037038012062884956 + pow2 64 * pow2 64 * 15197544864945402661 + pow2 64 * pow2 64 * pow2 64 * 9615747158586711429 < prime256);
   assert_norm (15992936863339206154 + pow2 64 * 10037038012062884956 + pow2 64 * pow2 64 * 15197544864945402661 + pow2 64 * pow2 64 * pow2 64 * 9615747158586711429 = 60359023176204190920225817201443260813112970217682417638161152432929735267850);
-  assert_norm (0x4FE342E2FE1A7F9B8EE7EB4A7C0F9E162BCE33576B315ECECBB6406837BF51F5 == fromDomain_ 60359023176204190920225817201443260813112970217682417638161152432929735267850);
+  assert_norm (0x4FE342E2FE1A7F9B8EE7EB4A7C0F9E162BCE33576B315ECECBB6406837BF51F5 == fromDomain_ #P256 60359023176204190920225817201443260813112970217682417638161152432929735267850);
   
   
   upd p (size 8) (u64 1);
@@ -638,12 +676,12 @@ let uploadBasePoint p =
   upd p (size 10) (u64 18446744073709551615);
   upd p (size 11) (u64 4294967294);
   assert_norm (1 + pow2 64 * 18446744069414584320 + pow2 64 * pow2 64 * 18446744073709551615 + pow2 64 * pow2 64 * pow2 64 * 4294967294 < prime256);
-  assert_norm (1 = fromDomain_ 26959946660873538059280334323183841250350249843923952699046031785985);
+  assert_norm (1 = fromDomain_ #P256 26959946660873538059280334323183841250350249843923952699046031785985);
   assert_norm (1 + pow2 64 * 18446744069414584320 + pow2 64 * pow2 64 * 18446744073709551615 + pow2 64 * pow2 64 * pow2 64 * 4294967294 = 26959946660873538059280334323183841250350249843923952699046031785985) 
 
 
-let scalarMultiplicationWithoutNorm p result scalar tempBuffer = 
-  let h0 = ST.get() in 
+let scalarMultiplicationWithoutNorm #c p result scalar tempBuffer = 
+  let h0 = ST.get() in  
   let q = sub tempBuffer (size 0) (size 12) in 
   uploadZeroPoint q;
   let buff = sub tempBuffer (size 12) (size 88) in 
@@ -652,33 +690,33 @@ let scalarMultiplicationWithoutNorm p result scalar tempBuffer =
   montgomery_ladder q result scalar buff;
   copy_point q result;  
     lemma_point_to_domain h0 h1 p result;
-    lemma_pif_to_domain h1 q
+    lemma_pif_to_domain #c h1 q
     
 
-let secretToPublic result scalar tempBuffer = 
+let secretToPublic #c result scalar tempBuffer = 
   push_frame(); 
     let basePoint = create (size 12) (u64 0) in 
-  uploadBasePoint basePoint;
+  uploadBasePoint #c basePoint;
     let q = sub tempBuffer (size 0) (size 12) in 
     let buff = sub tempBuffer (size 12) (size 88) in 
   uploadZeroPoint q; 
   let h1 = ST.get() in 
-    lemma_pif_to_domain h1 q;
-  montgomery_ladder q basePoint scalar buff; 
+    lemma_pif_to_domain #c h1 q;
+  montgomery_ladder #c q basePoint scalar buff; 
   norm q result buff;  
   pop_frame()
 
 
-let secretToPublicWithoutNorm result scalar tempBuffer = 
+let secretToPublicWithoutNorm #c result scalar tempBuffer = 
   push_frame(); 
     let basePoint = create (size 12) (u64 0) in 
-  uploadBasePoint basePoint;
+  uploadBasePoint #c basePoint;
       let q = sub tempBuffer (size 0) (size 12) in 
       let buff = sub tempBuffer (size 12) (size 88) in 
   uploadZeroPoint q; 
       let h1 = ST.get() in 
-      lemma_pif_to_domain h1 q; 
-  montgomery_ladder q basePoint scalar buff; 
+      lemma_pif_to_domain #c h1 q; 
+  montgomery_ladder #c q basePoint scalar buff; 
   copy_point q result;
   pop_frame()  
 
