code/ecdsap256/Hacl.Impl.P256.Core.fsti
@@ -23,21 +23,21 @@ module B = LowStar.Buffer
 open FStar.Mul
 
 inline_for_extraction noextract 
-val toDomain: value: felem -> result: felem ->  Stack unit 
-  (requires fun h ->  as_nat h value < prime256 /\ live h value /\live h result /\ eq_or_disjoint value result)
-  (ensures fun h0 _ h1 -> modifies (loc result) h0 h1 /\ as_nat h1 result = toDomain_ (as_nat h0 value))
+val toDomain: #c: curve -> value: felem c -> result: felem c ->  Stack unit 
+  (requires fun h ->  as_nat c h value < prime256 /\ live h value /\live h result /\ eq_or_disjoint value result)
+  (ensures fun h0 _ h1 -> modifies (loc result) h0 h1 /\ as_nat c h1 result = toDomain_ #c (as_nat c h0 value))
  
  
 inline_for_extraction noextract
-val fromDomain: f: felem-> result: felem-> Stack unit 
-  (requires fun h -> live h f /\ live h result /\ as_nat h f < prime256)
+val fromDomain: #c: curve -> f: felem c -> result: felem c -> Stack unit 
+  (requires fun h -> live h f /\ live h result /\ as_nat c h f < prime256)
   (ensures fun h0 _ h1 -> modifies (loc result) h0 h1 /\ 
-    as_nat h1 result = (as_nat h0 f * modp_inv2 #P256 (pow2 256)) % prime256 /\ 
-    as_nat h1 result = fromDomain_ (as_nat h0 f))
+    as_nat c h1 result = (as_nat c h0 f * modp_inv2 #c (pow2 256)) % prime256 /\ 
+    as_nat c h1 result = fromDomain_ #c (as_nat c h0 f))
 
 
 noextract 
-let point_x_as_nat (h: mem) (e: point) : GTot nat = 
+let point_x_as_nat (c: curve) (h: mem) (e: point c) : GTot nat = 
   let open Lib.Sequence in 
   let s = as_seq h e in 
   let s0 = s.[0] in
@@ -47,7 +47,7 @@ let point_x_as_nat (h: mem) (e: point) : GTot nat =
   as_nat4 (s0, s1, s2, s3)
 
 noextract 
-let point_y_as_nat (h: mem) (e: point) : GTot nat = 
+let point_y_as_nat (c: curve) (h: mem) (e: point c) : GTot nat = 
   let open Lib.Sequence in 
   let s = as_seq h e in 
   let s0 = s.[4] in
@@ -57,7 +57,7 @@ let point_y_as_nat (h: mem) (e: point) : GTot nat =
   as_nat4 (s0, s1, s2, s3)
 
 noextract 
-let point_z_as_nat (h: mem) (e: point) : GTot nat = 
+let point_z_as_nat (c: curve) (h: mem) (e: point c) : GTot nat = 
   let open Lib.Sequence in 
   let s = as_seq h e in 
   let s0 = s.[8] in
@@ -67,31 +67,31 @@ let point_z_as_nat (h: mem) (e: point) : GTot nat =
   as_nat4 (s0, s1, s2, s3)
 
 
-val pointToDomain: p: point -> result: point -> Stack unit 
+val pointToDomain: #c: curve -> p: point c -> result: point c -> Stack unit 
   (requires fun h -> live h p /\ live h result /\ eq_or_disjoint p result /\ 
-    point_x_as_nat h p < prime256 /\ point_y_as_nat h p < prime256 /\ point_z_as_nat h p < prime256)
+    point_x_as_nat c h p < prime256 /\ point_y_as_nat c h p < prime256 /\ point_z_as_nat c h p < prime256)
   (ensures fun h0 _ h1 -> modifies (loc result) h0 h1 /\ 
-    point_x_as_nat h1 result == toDomain_ (point_x_as_nat h0 p) /\
-    point_y_as_nat h1 result == toDomain_ (point_y_as_nat h0 p) /\
-    point_z_as_nat h1 result == toDomain_ (point_z_as_nat h0 p))
+    point_x_as_nat c h1 result == toDomain_ #c (point_x_as_nat c h0 p) /\
+    point_y_as_nat c h1 result == toDomain_ #c (point_y_as_nat c h0 p) /\
+    point_z_as_nat c h1 result == toDomain_ #c (point_z_as_nat c h0 p))
 
 
-val pointFromDomain: p: point -> result: point-> Stack unit 
+val pointFromDomain: #c : curve -> p: point c -> result: point c-> Stack unit 
   (requires fun h -> live h p /\ live h result /\ eq_or_disjoint p result /\ 
-  point_x_as_nat h p < prime256 /\ point_y_as_nat h p < prime256 /\ point_z_as_nat h p < prime256)
+  point_x_as_nat c h p < prime256 /\ point_y_as_nat c h p < prime256 /\ point_z_as_nat c h p < prime256)
   (ensures fun h0 _ h1 -> modifies (loc result) h0 h1 /\
-    point_x_as_nat h1 result == fromDomain_ (point_x_as_nat h0 p) /\
-    point_y_as_nat h1 result == fromDomain_ (point_y_as_nat h0 p) /\
-    point_z_as_nat h1 result == fromDomain_ (point_z_as_nat h0 p))
+    point_x_as_nat c h1 result == fromDomain_ #c (point_x_as_nat c h0 p) /\
+    point_y_as_nat c h1 result == fromDomain_ #c (point_y_as_nat c h0 p) /\
+    point_z_as_nat c h1 result == fromDomain_ #c (point_z_as_nat c h0 p))
     
 
-val isPointAtInfinityPrivate: p: point -> Stack uint64
-  (requires fun h -> live h p /\ as_nat h (gsub p (size 8) (size 4)) < prime256)
+val isPointAtInfinityPrivate: #c: curve -> p: point c -> Stack uint64
+  (requires fun h -> live h p /\ as_nat c h (gsub p (size 8) (size 4)) < prime256)
   (ensures fun h0 r h1 -> modifies0 h0 h1 /\      
     (
       (uint_v r == 0 \/ uint_v r == maxint U64) /\ 
       (
-	let x, y, z = fromDomainPoint(point_prime_to_coordinates (as_seq h0 p)) in 
+	let x, y, z = fromDomainPoint #c (point_prime_to_coordinates (as_seq h0 p)) in 
 	if Spec.P256.isPointAtInfinity (x, y, z) then uint_v r = maxint U64 else uint_v r = 0
       ) /\
       (
@@ -101,98 +101,98 @@ val isPointAtInfinityPrivate: p: point -> Stack uint64
    )
   )
 
-val norm: p: point -> resultPoint: point -> tempBuffer: lbuffer uint64 (size 88) -> Stack unit
+val norm: #c: curve -> p: point c -> resultPoint: point c -> tempBuffer: lbuffer uint64 (size 88) -> Stack unit
   (requires fun h -> live h p /\ live h resultPoint /\ live h tempBuffer /\ disjoint p tempBuffer /\ disjoint tempBuffer resultPoint /\ 
-    as_nat h (gsub p (size 0) (size 4)) < prime256 /\
-    as_nat h (gsub p (size 4) (size 4)) < prime256 /\
-    as_nat h (gsub p (size 8) (size 4)) < prime256 
+    as_nat c h (gsub p (size 0) (size 4)) < prime256 /\
+    as_nat c h (gsub p (size 4) (size 4)) < prime256 /\
+    as_nat c h (gsub p (size 8) (size 4)) < prime256 
   ) 
   (ensures fun h0 _ h1 -> 
       modifies (loc tempBuffer |+| loc resultPoint) h0 h1 /\
       (
       let resultPoint =  point_prime_to_coordinates (as_seq h1 resultPoint) in 
-      let pointD = fromDomainPoint (point_prime_to_coordinates (as_seq h0 p)) in 
+      let pointD = fromDomainPoint #c (point_prime_to_coordinates (as_seq h0 p)) in 
       let pointNorm = _norm #P256 pointD in 
       pointNorm == resultPoint
    )   
   )
 
 
-val normX: p: point -> result: felem -> tempBuffer: lbuffer uint64 (size 88) -> Stack unit
+val normX: #c: curve -> p: point c -> result: felem c -> tempBuffer: lbuffer uint64 (size 88) -> Stack unit
   (requires fun h -> live h p /\ live h result /\ live h tempBuffer /\
     LowStar.Monotonic.Buffer.all_disjoint [loc p; loc result; loc tempBuffer] /\ 
-    as_nat h (gsub p (size 0) (size 4)) < prime256 /\
-    as_nat h (gsub p (size 4) (size 4)) < prime256 /\
-    as_nat h (gsub p (size 8) (size 4)) < prime256 
+    as_nat c h (gsub p (size 0) (size 4)) < prime256 /\
+    as_nat c h (gsub p (size 4) (size 4)) < prime256 /\
+    as_nat c h (gsub p (size 8) (size 4)) < prime256 
   ) 
   (ensures fun h0 _ h1 -> 
       modifies (loc tempBuffer |+| loc result) h0 h1  /\
       (
-	let pxD = fromDomain_ (as_nat h0 (gsub p (size 0) (size 4))) in 
-	let pyD = fromDomain_ (as_nat h0 (gsub p (size 4) (size 4))) in 
-	let pzD = fromDomain_ (as_nat h0 (gsub p (size 8) (size 4))) in 
+	let pxD = fromDomain_ #c (as_nat c h0 (gsub p (size 0) (size 4))) in 
+	let pyD = fromDomain_ #c (as_nat c h0 (gsub p (size 4) (size 4))) in 
+	let pzD = fromDomain_ #c (as_nat c h0 (gsub p (size 8) (size 4))) in 
       
 	let (xN, _, _) = _norm #P256 (pxD, pyD, pzD) in 
-	as_nat h1 result == xN
+	as_nat c h1 result == xN
       )
   )
 
 
 
 inline_for_extraction noextract
-val scalarMultiplication: #buf_type: buftype->  p: point -> result: point -> 
+val scalarMultiplication: #c: curve -> #buf_type: buftype->  p: point c -> result: point c -> 
   scalar: lbuffer_t buf_type uint8 (size 32) -> 
   tempBuffer: lbuffer uint64 (size 100) ->
   Stack unit
     (requires fun h -> 
       live h p /\ live h result /\ live h scalar /\ live h tempBuffer /\
     LowStar.Monotonic.Buffer.all_disjoint [loc p; loc tempBuffer; loc scalar; loc result] /\
-    as_nat h (gsub p (size 0) (size 4)) < prime256 /\ 
-    as_nat h (gsub p (size 4) (size 4)) < prime256 /\
-    as_nat h (gsub p (size 8) (size 4)) < prime256
+    as_nat c h (gsub p (size 0) (size 4)) < prime256 /\ 
+    as_nat c h (gsub p (size 4) (size 4)) < prime256 /\
+    as_nat c h (gsub p (size 8) (size 4)) < prime256
     )
   (ensures fun h0 _ h1 -> 
     modifies3 p result tempBuffer h0 h1 /\ 
     modifies (loc p |+| loc result |+| loc tempBuffer) h0 h1 /\
-    as_nat h1 (gsub result (size 0) (size 4)) < prime256 /\ 
-    as_nat h1 (gsub result (size 4) (size 4)) < prime256 /\
-    as_nat h1 (gsub result (size 8) (size 4)) < prime256 /\
+    as_nat c h1 (gsub result (size 0) (size 4)) < prime256 /\ 
+    as_nat c h1 (gsub result (size 4) (size 4)) < prime256 /\
+    as_nat c h1 (gsub result (size 8) (size 4)) < prime256 /\
     (
-      let x3, y3, z3 = point_x_as_nat h1 result, point_y_as_nat h1 result, point_z_as_nat h1 result in 
+      let x3, y3, z3 = point_x_as_nat c h1 result, point_y_as_nat c h1 result, point_z_as_nat c h1 result in 
       let (xN, yN, zN) = scalar_multiplication #P256 (as_seq h0 scalar) (point_prime_to_coordinates (as_seq h0 p)) in 
       x3 == xN /\ y3 == yN /\ z3 == zN 
   )
 ) 
 
 
-val scalarMultiplicationWithoutNorm: p: point -> result: point -> 
+val scalarMultiplicationWithoutNorm: #c: curve -> p: point c -> result: point c -> 
   scalar: lbuffer  uint8 (size 32) -> 
   tempBuffer: lbuffer uint64 (size 100) ->
   Stack unit
     (requires fun h -> 
       live h p /\ live h result /\ live h scalar /\ live h tempBuffer /\
     LowStar.Monotonic.Buffer.all_disjoint [loc p; loc tempBuffer; loc scalar; loc result] /\
-    as_nat h (gsub p (size 0) (size 4)) < prime256 /\ 
-    as_nat h (gsub p (size 4) (size 4)) < prime256 /\
-    as_nat h (gsub p (size 8) (size 4)) < prime256
+    as_nat c h (gsub p (size 0) (size 4)) < prime256 /\ 
+    as_nat c h (gsub p (size 4) (size 4)) < prime256 /\
+    as_nat c h (gsub p (size 8) (size 4)) < prime256
     )
   (ensures fun h0 _ h1 -> 
     modifies (loc p |+| loc result |+| loc tempBuffer) h0 h1 /\ 
     
-    as_nat h1 (gsub result (size 0) (size 4)) < prime256 /\ 
-    as_nat h1 (gsub result (size 4) (size 4)) < prime256 /\
-    as_nat h1 (gsub result (size 8) (size 4)) < prime256 /\
+    as_nat c h1 (gsub result (size 0) (size 4)) < prime256 /\ 
+    as_nat c h1 (gsub result (size 4) (size 4)) < prime256 /\
+    as_nat c h1 (gsub result (size 8) (size 4)) < prime256 /\
     
     modifies (loc p |+| loc result |+| loc tempBuffer) h0 h1 /\
     (
-      let p1 = fromDomainPoint(point_prime_to_coordinates (as_seq h1 result)) in 
+      let p1 = fromDomainPoint #c (point_prime_to_coordinates (as_seq h1 result)) in 
       let rN, _ = montgomery_ladder_spec #P256 (as_seq h0 scalar) ((0, 0, 0),  point_prime_to_coordinates (as_seq h0 p)) in 
       rN == p1
   )
 ) 
 
 
-val secretToPublic: result: point -> scalar: lbuffer uint8 (size 32) -> tempBuffer: lbuffer uint64 (size 100) ->
+val secretToPublic: #c: curve -> result: point c  -> scalar: lbuffer uint8 (size 32) -> tempBuffer: lbuffer uint64 (size 100) ->
   Stack unit
     (requires fun h -> 
       live h result /\ live h scalar /\ live h tempBuffer /\ 
@@ -200,17 +200,17 @@ val secretToPublic: result: point -> scalar: lbuffer uint8 (size 32) -> tempBuff
     )
   (
     ensures fun h0 _ h1 -> modifies (loc result |+| loc tempBuffer) h0 h1 /\
-    as_nat h1 (gsub result (size 0) (size 4)) < prime256 /\ 
-    as_nat h1 (gsub result (size 4) (size 4)) < prime256 /\ 
-    as_nat h1 (gsub result (size 8) (size 4)) < prime256 /\
+    as_nat c h1 (gsub result (size 0) (size 4)) < prime256 /\ 
+    as_nat c h1 (gsub result (size 4) (size 4)) < prime256 /\ 
+    as_nat c h1 (gsub result (size 8) (size 4)) < prime256 /\
     (
-      let x3, y3, z3 = point_x_as_nat h1 result, point_y_as_nat h1 result, point_z_as_nat h1 result in 
+      let x3, y3, z3 = point_x_as_nat c h1 result, point_y_as_nat c h1 result, point_z_as_nat c h1 result in 
       let (xN, yN, zN) = secret_to_public #P256 (as_seq h0 scalar)  in 
       x3 == xN /\ y3 == yN /\ z3 == zN 
     )
   )
 
-val secretToPublicWithoutNorm: result: point -> scalar: lbuffer uint8 (size 32) -> 
+val secretToPublicWithoutNorm: #c: curve -> result: point c -> scalar: lbuffer uint8 (size 32) -> 
  tempBuffer: lbuffer uint64 (size 100) ->
   Stack unit
     (requires fun h -> 
@@ -219,10 +219,10 @@ val secretToPublicWithoutNorm: result: point -> scalar: lbuffer uint8 (size 32) 
     )
   (
     ensures fun h0 _ h1 -> modifies (loc result |+| loc tempBuffer) h0 h1 /\
-      as_nat h1 (gsub result (size 0) (size 4)) < prime256 /\ 
-      as_nat h1 (gsub result (size 4) (size 4)) < prime256 /\ 
-      as_nat h1 (gsub result (size 8) (size 4)) < prime256 /\
+      as_nat c h1 (gsub result (size 0) (size 4)) < prime256 /\ 
+      as_nat c h1 (gsub result (size 4) (size 4)) < prime256 /\ 
+      as_nat c h1 (gsub result (size 8) (size 4)) < prime256 /\
       (
-	let p1 = fromDomainPoint(point_prime_to_coordinates (as_seq h1 result)) in 
+	let p1 = fromDomainPoint #c (point_prime_to_coordinates (as_seq h1 result)) in 
 	let rN, _ = montgomery_ladder_spec (as_seq h0 scalar) ((0, 0, 0), (basePoint #P256)) in 
 	rN == p1))  
